timesyn/CaseStudies/abp/MediumRSAutomaton.thy
@@ -1,58 +1,47 @@
-
-
+(*
+ * DO NOT MODIFY!
+ * This file was generated from MediumRS.maa and will be overridden when changed. To change
+ * permanently, consider changing the model itself.
+ *
+ * Generated on Jun 29, 2018 5:23:56 PM by transformer 1.0.0
+ *)
 theory MediumRSAutomaton
 
-imports "../AutomatonPrelude"
+imports "../AutomatonPrelude" "../../../untimed/CaseStudy/NDA"
 
 begin
 
 (* This are the actual states from MAA *)
 datatype MediumRSSubstate = Single
 
-(* SWS: ins kommentar davor wie die Variable heißt *)
 (* And these have also the variables *)
-datatype MediumRSState = State MediumRSSubstate (* SWS: c=*)"nat"
+datatype MediumRSState = State MediumRSSubstate (* c = *) "nat"
 
 fun getSubState :: "MediumRSState \<Rightarrow> MediumRSSubstate" where
-    "getSubState (State state_s automaton_c) = state_s"
+"getSubState (State state_s automaton_c) = state_s"
 
 fun getC :: "MediumRSState \<Rightarrow> nat" where
 "getC (State _ automaton_c) = automaton_c"
     
 
-(* SWS: siehe receiver *)
-abbreviation input_ar_c4 :: "channel" ("\<guillemotright>ar") where
-"\<guillemotright>ar \<equiv> c4"
 
-abbreviation output_as_c1 :: "channel" ("as\<guillemotright>") where
-"as\<guillemotright> \<equiv> c1"
+fun mediumRSTransitionH :: "(MediumRSState \<times> (abpMessage tsyn)) \<Rightarrow> ((MediumRSState \<times> abpMessage tsyn SB) set rev)" where
+    "mediumRSTransitionH (State Single automaton_c, ((*ar\<mapsto>*)Msg (Bool a))) = 
+       (if(automaton_c=0) then Rev {(State Single (c),(tsynbNull (\<C> ''as'')))| (c). (c) < 50}
+       else if(automaton_c>0) then Rev {(State Single (automaton_c-1),(tsynbNull (\<C> ''as'')))}
+       else if(True) then Rev {(State Single automaton_c,(tsynbNull (\<C> ''as'')))}
+       else Rev {(State Single automaton_c, ((tsynbNull (\<C> ''as''))))})"  |
 
-(* SWS: siehe receiver *)
-lift_definition createAsOutput :: "bool \<Rightarrow> Message tsyn SB" is
-    "\<lambda>b. [ as\<guillemotright> \<mapsto> \<up>(Msg (bool b))]"
-unfolding ubWell_def
-unfolding usclOkay_stream_def
-unfolding ctype_tsyn_def
-by simp
+    "mediumRSTransitionH (State Single automaton_c, ((*ar\<mapsto>*)null)) = 
+       (Rev {(State Single automaton_c,(tsynbNull (\<C> ''as'')))})"  
 
-(* SWS: Das Medium ist nichtdeterministisch, siehe das Beispiel in "untimed/CaseStudy/Medium.thy" *)
-fun mediumRSTransitionH :: "(MediumRSState \<times> (Message tsyn)) \<Rightarrow> (MediumRSState \<times> Message tsyn SB)" where
-    "mediumRSTransitionH (State Single automaton_c, (Msg (bool a))) = 
-       (if(automaton_c=0) then ((State Single (50),(tsynbNull as\<guillemotright>)))
-       else if(automaton_c>0) then ((State Single (automaton_c-1),(tsynbNull as\<guillemotright>)))
-       else if(True) then ((State Single automaton_c,(tsynbNull as\<guillemotright>)))
-       else  (State Single automaton_c, ((tsynbNull as\<guillemotright>))))"  |
+fun mediumRSTransition :: "(MediumRSState \<times> (channel \<rightharpoonup> abpMessage tsyn)) \<Rightarrow> ((MediumRSState \<times> abpMessage tsyn SB) set rev)" where
+"mediumRSTransition (s,f) = (if dom(f) = {\<C> ''ar''} then mediumRSTransitionH (s,(f\<rightharpoonup>\<C> ''ar'')) else undefined)"
 
-    "mediumRSTransitionH (State Single automaton_c, (null)) = 
-       (State Single automaton_c,(tsynbNull as\<guillemotright>))"  
+lift_definition MediumRSAutomaton :: "(MediumRSState, abpMessage tsyn) NDA" is "(mediumRSTransition, Rev {(State Single c, (tsynbNull (\<C> ''as'')))| c. c < 50}, Discr {\<C> ''ar''}, Discr {\<C> ''as''})"
+  by simp
 
-fun mediumRSTransition :: "(MediumRSState \<times> (channel \<rightharpoonup> Message tsyn)) \<Rightarrow> (MediumRSState \<times> Message tsyn SB)" where
-"mediumRSTransition (s,f) = (if dom(f) = {\<guillemotright>ar} then mediumRSTransitionH (s,(f\<rightharpoonup>\<guillemotright>ar)) else undefined)"
-
-lift_definition MediumRSAutomaton :: "(MediumRSState, Message tsyn) automaton" is "(mediumRSTransition, State Single 50, (tsynbNull as\<guillemotright>), {c4}, {c1})"
-sorry
-
-definition MediumRSSPF :: "Message tsyn SPF" where
-"MediumRSSPF = H MediumRSAutomaton"
+definition MediumRSSPF :: "abpMessage tsyn SPS" where
+"MediumRSSPF = nda_H\<cdot>MediumRSAutomaton"
 
 end
